

## S.4 Comparison Tests

Ex1  $\sum_{n=1}^{\infty} \frac{\cos^2 n}{n^2}$   $a_n = \frac{\cos^2 n}{n^2}$  . What should  $b_n$  be?

(usually  $b_n = \frac{1}{n^p}$  works as a p-series.)

$$0 \leq \cos^2 n \leq 1$$

Try  $b_n = \frac{1}{n^2}$

(1) Make comparison 
$$0 \leq \frac{\cos^2 n}{n^2} \leq \frac{1}{n^2}$$
  
" " " "  
 $a_n \quad b_n$

(2) Note  $\sum b_n = \sum \frac{1}{n^2}$  converges by p-series since  $p=2>1$ .

(3) Thus  $\sum a_n = \sum \frac{\cos^2 n}{n^2}$  converges by Comparison Test.

---

Ex2  $a_n = \frac{\sin(\frac{1}{n})}{\sqrt{n}}$  . Determine whether  $\sum a_n$

converges or diverges.

Try Divergence Test: as  $n \rightarrow \infty$   $\sin(\frac{1}{n}) \rightarrow \sin(0) = 0$   
 $\frac{1}{\sqrt{n}} \rightarrow 0$

$$a_n \rightarrow 0 \cdot 0 = 0$$

Divergence Test does not apply.

Series may converge, or not.

$$\lim_{x \rightarrow 0^+} \frac{\sin x}{x} = 1 = \lim_{n \rightarrow \infty} \frac{\sin(\frac{1}{n})}{(\frac{1}{n})} \quad *$$

$$x = \frac{1}{n}$$

$$n \rightarrow \infty$$

$$\frac{\sin(\frac{1}{n})}{(\frac{1}{n})} < 1$$

get  $\frac{\sin(\frac{1}{n})}{\sqrt{n}}$   
multiply by  $\frac{1}{n^{3/2}}$   
on both sides

$$\Leftrightarrow n \cdot \sin(\frac{1}{n}) < 1$$

$$\Leftrightarrow \frac{1}{n^{3/2}} \cdot n \cdot \sin(\frac{1}{n}) < \frac{1}{n^{3/2}}$$

$$\Leftrightarrow a_n = \frac{\sin(\frac{1}{n})}{\sqrt{n}} < \frac{1}{n^{3/2}} = b_n \quad (1)$$

By p-series,  $p = \frac{3}{2} > 1$ ,  $\sum b_n$  converges. (2)

By Comparison Test, since  $a_n < b_n$  as  $n \rightarrow \infty$   
(for all  $n \geq N$ ) we have that  $\sum a_n$  converges (3)

Exercise for you Ex 3  $\sum \frac{1}{n+1}$ .  $a_n = \frac{1}{n+1}$ .

Should  $b_n = \frac{1}{n}$  or  $b_n = \frac{1}{2n}$ .

And do these series converge or diverge??

## Limit Comparison Test

Ex 4  $\sum_{n=2}^{\infty} \frac{\ln n}{n^2}$   $a_n = \frac{\ln n}{n^2}$

$\ln n \ll n^2$  so by growth rates  $\frac{\ln n}{n^2} \rightarrow 0$

So Divergence Test gives no info on this series.

Choose  $b_n$  (1) option  $b_n = \frac{1}{n^2}$

$$\frac{a_n}{b_n} = \left( \frac{\ln n}{n^2} \right) \times \frac{n^2}{1} = \ln n \rightarrow \infty \quad \times \quad \text{does not show convergence}$$

$$\frac{a_n}{b_n} > M \Rightarrow a_n > M b_n$$

So  $a_n$  terms are bigger than terms of a convergent series

$\Rightarrow$  NO INFO.

(2) option  $b_n = \frac{1}{n^{1.1}}$

$$\frac{a_n}{b_n} = \left( \frac{\ln n}{n^2} \right) \left( \frac{n^{1.1}}{1} \right) = \frac{\ln n}{n^{0.9}} \rightarrow 0 \quad (1)$$

by  $\ln n \ll n^{0.9}$

$$\frac{a_n}{b_n} < \varepsilon$$

$$a_n < b_n \cdot \varepsilon \quad (\text{proof ...})$$

so  $a_n$  terms are smaller than terms of a convergent series.

By Limit comparison Test, since  $\frac{a_n}{b_n} \rightarrow 0$

and  $\sum_1^{\infty} b_n = \sum_1^{\infty} \frac{1}{n^{1.1}}$  converges by p-series (2)

$$p = 1.1 > 1$$

we conclude  $\sum_1^{\infty} a_n = \sum_1^{\infty} \frac{\ln n}{n^2}$  converges. (3)

Ex 5 (1)  $\sum_1^{\infty} \frac{n^0}{n^2+1}$   $\frac{n^1}{n^2} = \frac{1}{n} = b_n$  What  $b_n$ ?

(2)  $\sum_1^{\infty} \frac{n^0+1}{n^3-1}$   $\frac{n^1}{n^3} = \frac{1}{n^2} = b_n$

D.O. (1)  $\frac{a_n}{b_n} = \frac{n}{n^2+1} \times \frac{n}{1} = \frac{n^2}{n^2+1} \rightarrow \frac{1}{1} = 1 = L \neq 0$

bc 1 is the ratio of the leading coefficients,  
and deg numer = deg denom.

By Limit Comp Test  $\sum_1^{\infty} a_n$   $\sum_1^{\infty} b_n$  either  
(3) { both converge, or  
both diverge

②  $\sum b_n = \sum \frac{1}{n}$  diverges by p-series  $p=1 \neq 1$ .

③ Therefore  $\sum a_n = \sum \frac{n}{n^2+1}$  diverges as well.

Pls try ②.

Benefits of LC in ① To establish divergence  
using  $b_n = \frac{1}{n}$  would need

$$b_n < a_n \quad \text{i.e.}$$

$$\frac{1}{n} < \frac{n}{n^2+1} \quad \Leftrightarrow$$

$$n^2+1 < n^2 \quad \underline{\underline{\text{false}}}.$$

So a more nuanced  $b_n$  is required.

$$\text{like } b_n = \frac{1}{2n}.$$

$\sum \frac{1}{2n}$  diverges bc it is a constant multiple of

$\sum \frac{1}{n}$ , which diverges.

$$\frac{1}{2n} = b_n < a_n = \frac{n}{n^2+1} \quad \Leftrightarrow$$

$$\frac{n^2+1}{-n^2} < \frac{2n^2}{-n^2} \quad \Leftrightarrow$$

$$1 < n^2 \quad \underline{\text{true}}.$$

Using  $b_n = \frac{1}{2n}$ , CT can be used to show

$\sum a_n$  diverges.

---